chore: cleanup

Iris/Iris/Instances/Lib/GhostMap.lean
@@ -30,8 +30,7 @@ variable [UFraction F] [LawfulFiniteMap H K] [GhostMapG GF F K V H]
 
 @[rocq_alias ghost_map_auth]
 public def ghost_map_auth (γ : GName) (dq : DFrac F) (m : H V) : IProp GF :=
-  iOwn (E := GhostMapG.elem) γ
-    (Auth dq (Std.PartialMap.map (fun x ↦ toAgree ⟨x⟩) m))
+  iOwn (E := GhostMapG.elem) γ (Auth dq (Std.PartialMap.map (fun x ↦ toAgree ⟨x⟩) m))
 
 #rocq_ignore ghost_map_auth_def "Not needed"
 #rocq_ignore ghost_map_auth_aux "Not needed"
@@ -40,6 +39,7 @@ public def ghost_map_auth (γ : GName) (dq : DFrac F) (m : H V) : IProp GF :=
 @[rocq_alias ghost_map_elem]
 public def ghost_map_elem (γ : GName) (dq : DFrac F) (k : K) (v : V) : IProp GF :=
   iOwn (E := GhostMapG.elem) γ (Frag k dq (toAgree ⟨v⟩))
+
 #rocq_ignore ghost_map_elem_def "Not needed"
 #rocq_ignore ghost_map_elem_aux "Not needed"
 #rocq_ignore ghost_map_elem_unseal "Not needed"
@@ -59,6 +59,8 @@ section lemmas
 variable {F K V : Type _} {H : Type _ → Type _} [UFraction F] [LawfulFiniteMap H K]
 variable [GhostMapG GF F K V H]
 
+open LawfulPartialMap
+
 @[rocq_alias ghost_map_elem_timeless]
 instance (γ : GName) (k : K) (dq : DFrac F) (v : V) :
     Timeless (PROP := IProp GF) (γ ↪◯MAP[k]{dq} v) := by
@@ -66,14 +68,13 @@ instance (γ : GName) (k : K) (dq : DFrac F) (v : V) :
   infer_instance
 
 @[rocq_alias ghost_map_elem_persistent]
-instance (γ : GName) (k : K) (v : V) :
-    Persistent (PROP := IProp GF) (γ ↪◯MAP[k]{.discard} v) := by
+instance (γ : GName) (k : K) (v : V) : Persistent (PROP := IProp GF) (γ ↪◯MAP[k]{.discard} v) := by
   unfold ghost_map_elem
   infer_instance
 
 @[rocq_alias ghost_map_elem_fractional]
-instance ghost_map_elem_fractional (γ : GName) (k : K) (v : V)
-    : Fractional (PROP := IProp GF) (fun q : F => γ ↪◯MAP[k]{.own q} v) where
+instance ghost_map_elem_fractional (γ : GName) (k : K) (v : V) :
+    Fractional (PROP := IProp GF) (fun q : F => γ ↪◯MAP[k]{.own q} v) where
   fractional p q := by
     unfold ghost_map_elem
     refine .trans ?_ iOwn_op
@@ -83,24 +84,23 @@ instance ghost_map_elem_fractional (γ : GName) (k : K) (v : V)
     exact Agree.idemp.symm
 
 @[rocq_alias ghost_map_elem_as_fractional]
-instance (γ : GName) (k : K) (v : V)
-    : AsFractional (PROP := IProp GF) (γ ↪◯MAP[k]{.own q} v)
-      (fun q => γ ↪◯MAP[k]{.own q} v) q where
+instance (γ : GName) (k : K) (v : V) : AsFractional (PROP := IProp GF) (γ ↪◯MAP[k]{.own q} v)
+    (fun q => γ ↪◯MAP[k]{.own q} v) q where
   as_fractional := IProp.ext_iff.mp rfl
   as_fractional_fractional := ghost_map_elem_fractional γ k v
 
 @[rocq_alias ghost_map_elems_unseal]
 theorem ghost_map_elems_unseal [DecidableEq K] γ (m : H V) dq :
-  ([∗map] k ↦ v ∈ m, γ ↪◯MAP[k]{dq} v) ==∗
-  iOwn (GF := GF) (E := GhostMapG.elem) γ ([^ op map] k ↦ v ∈ m,
-    Frag k dq (toAgree (⟨v⟩: LeibnizO V))) := by
+    ([∗map] k ↦ v ∈ m, γ ↪◯MAP[k]{dq} v) ==∗
+    iOwn (GF := GF) (E := GhostMapG.elem) γ ([^ op map] k ↦ v ∈ m,
+      Frag k dq (toAgree (⟨v⟩: LeibnizO V))) := by
   iintro H
   by_cases h : m ≡ₘ ∅
   · iapply OFE.NonExpansive.eqv <| OFE.NonExpansive.eqv (BigOpM.bigOpM_equiv_of_perm _ h)
-    simp [BigOpM.bigOpM_empty]
+    simp only [BigOpM.bigOpM_empty]
     iapply iOwn_unit (γ := γ) (ε := unit)
   · imodintro
-    iapply bigOpM_iOwn _ _ _ (fun c => h c)
+    iapply bigOpM_iOwn _ _ _ h
     unfold ghost_map_elem
     iexact H
 
@@ -108,8 +108,8 @@ theorem ghost_map_elems_unseal [DecidableEq K] γ (m : H V) dq :
 theorem ghost_map_elem_valid (γ : GName) (k : K) (dq : DFrac F) (v : V) :
     (γ ↪◯MAP[k]{dq} v) ⊢@{IProp GF} internalCmraValid dq := by
   refine iOwn_cmraValid.trans ?_
-  iintro h
-  ipure h; ipure_intro
+  iintro %h
+  ipure_intro
   exact (frag_valid_iff.mp h).left
 
 @[rocq_alias ghost_map_elem_valid_2]
@@ -131,9 +131,9 @@ theorem ghost_map_elem_agree (γ : GName) (k : K) (dq1 dq2 : DFrac F) (v1 v2 : V
 
 @[rocq_alias ghost_map_elem_combine_gives]
 instance ghost_map_elem_combine_gives γ (k : K) (dq1 dq2 : DFrac F) (v1 v2 : V) :
-  CombineSepGives (PROP := IProp GF)
-    (γ ↪◯MAP[k]{dq1} v1) (γ ↪◯MAP[k]{dq2} v2)
-    iprop(⌜✓ (dq1 • dq2) ∧ v1 = v2⌝) where
+    CombineSepGives (PROP := IProp GF)
+      (γ ↪◯MAP[k]{dq1} v1) (γ ↪◯MAP[k]{dq2} v2)
+      iprop(⌜✓ (dq1 • dq2) ∧ v1 = v2⌝) where
   combine_sep_gives := by
     iintro H
     icases ghost_map_elem_valid_2 $$ H with %H
@@ -141,8 +141,8 @@ instance ghost_map_elem_combine_gives γ (k : K) (dq1 dq2 : DFrac F) (v1 v2 : V)
 
 @[rocq_alias ghost_map_elem_combine]
 theorem ghost_map_elem_combine (γ : GName) (k : K) (dq1 dq2 : DFrac F) (v1 v2 : V) :
-    ⊢@{IProp GF}(γ ↪◯MAP[k]{dq1} v1) -∗ (γ ↪◯MAP[k]{dq2} v2)
-      -∗ (γ ↪◯MAP[k]{dq1 • dq2} v1) ∗ ⌜v1 = v2⌝ := by
+    ⊢@{IProp GF}(γ ↪◯MAP[k]{dq1} v1) -∗ (γ ↪◯MAP[k]{dq2} v2) -∗
+      (γ ↪◯MAP[k]{dq1 • dq2} v1) ∗ ⌜v1 = v2⌝ := by
   iintro Hl1 Hl2
   icases ghost_map_elem_agree $$ [$Hl1 $Hl2] with #%heq
   iframe %heq; subst heq
@@ -151,26 +151,25 @@ theorem ghost_map_elem_combine (γ : GName) (k : K) (dq1 dq2 : DFrac F) (v1 v2 :
 
 @[rocq_alias ghost_map_elem_combine_as]
 instance ghost_map_elem_combine_as (γ : GName) (k : K) (dq1 dq2 : DFrac F) (v1 v2 : V) :
-  CombineSepAs (PROP := IProp GF)
-    (γ ↪◯MAP[k]{dq1} v1) (γ ↪◯MAP[k]{dq2} v2)
-    (γ ↪◯MAP[k]{dq1 • dq2} v1) where
+    CombineSepAs (PROP := IProp GF)
+      (γ ↪◯MAP[k]{dq1} v1) (γ ↪◯MAP[k]{dq2} v2)
+      (γ ↪◯MAP[k]{dq1 • dq2} v1) where
   combine_sep_as := by
     iintro ⟨Hl1, Hl2⟩
     icases ghost_map_elem_combine $$ Hl1 Hl2 with ⟨H, -⟩
     iframe
 
 @[rocq_alias ghost_map_elem_frac_ne]
-theorem ghost_map_elem_frac_ne γ (k1 k2 : K) (dq1 dq2 : DFrac F) (v1 v2 : V) :
-   ¬ ✓ (dq1 • dq2) →
+theorem ghost_map_elem_frac_ne γ (k1 k2 : K) (dq1 dq2 : DFrac F) (v1 v2 : V) (Hk : ¬ ✓ (dq1 • dq2)) :
     ⊢@{IProp GF} (γ ↪◯MAP[k1]{dq1} v1) -∗ (γ ↪◯MAP[k2]{dq2} v2) -∗ ⌜k1 ≠ k2⌝ := by
-  iintro %Hcontra Hl1 Hl2
+  iintro Hl1 Hl2
   iintro %Heq; subst Heq
   icombine Hl1 Hl2 gives ⟨%_, %_⟩
   trivial
 
 @[rocq_alias ghost_map_elem_ne]
 theorem ghost_map_elem_ne γ (k1 k2 : K) (dq : DFrac F) (v1 v2 : V) :
-  ⊢@{IProp GF} (γ ↪◯MAP[k1] v1) -∗ (γ ↪◯MAP[k2]{dq} v2) -∗ ⌜k1 ≠ k2⌝ := by
+    ⊢@{IProp GF} (γ ↪◯MAP[k1] v1) -∗ (γ ↪◯MAP[k2]{dq} v2) -∗ ⌜k1 ≠ k2⌝ := by
   iintro H G
   iapply ghost_map_elem_frac_ne $$ H G
   intro HContra
@@ -179,7 +178,7 @@ theorem ghost_map_elem_ne γ (k1 k2 : K) (dq : DFrac F) (v1 v2 : V) :
 /-- Make an element read-only. -/
 @[rocq_alias ghost_map_elem_persist]
 theorem ghost_map_elem_persist (γ : GName) (k : K) (dq : DFrac F) (v : V) :
-  ⊢@{IProp GF} (γ ↪◯MAP[k]{dq} v) ==∗ (γ ↪◯MAP[k]{.discard} v) := by
+    ⊢@{IProp GF} (γ ↪◯MAP[k]{dq} v) ==∗ (γ ↪◯MAP[k]{.discard} v) := by
   unfold ghost_map_elem
   iintro H
   iapply iOwn_update $$ H
@@ -188,7 +187,7 @@ theorem ghost_map_elem_persist (γ : GName) (k : K) (dq : DFrac F) (v : V) :
 /-- Recover fractional ownership for a read-only element. -/
 @[rocq_alias ghost_map_elem_unpersist]
 theorem ghost_map_elem_unpersist [IsHalfFraction F] (γ : GName) (k : K) (v : V) :
-  ⊢@{IProp GF} (γ ↪◯MAP[k]{.discard} v) ==∗ ∃ q, (γ ↪◯MAP[k]{.own q} v) := by
+    ⊢@{IProp GF} (γ ↪◯MAP[k]{.discard} v) ==∗ ∃ q, (γ ↪◯MAP[k]{.own q} v) := by
   unfold ghost_map_elem
   iintro H
   imod iOwn_updateP update_frag_acquire $$ H with ⟨%a, %Heq, G⟩
@@ -205,47 +204,37 @@ theorem ghost_map_alloc_strong [DecidableEq K] (P : GName → Prop) (m : H V) :
   unfold ghost_map_elem ghost_map_auth
   iintro %Hinf
   imod iOwn_alloc_strong (E := GhostMapG.elem)
-    (Auth (DFrac.own 1) (K := K) (V := (Agree (LeibnizO V))) (Std.PartialMap.map (fun x => toAgree ⟨x⟩) ∅)) P Hinf with ⟨%γ, %HP, G⟩
+    (Auth (DFrac.own 1) (V := Agree (LeibnizO V)) (∅ : H _)) P Hinf with ⟨%γ, %HP, G⟩
   · simpa only [auth_valid_iff] using DFrac.valid_own_one
   · iexists γ; iframe %HP
-    iapply BIUpdate.mono <| sep_mono_r <|
-      bigOpM_iOwn_entail (F := constOF (HeapView F K (Agree (LeibnizO V)) H))
-        (E := GhostMapG.elem) γ _ m
+    iapply BIUpdate.mono <| sep_mono_r <| bigOpM_iOwn_entail γ _ m
     iapply BIUpdate.mono <| iOwn_op.mp
     iapply iOwn_update $$ G
-    refine Update.equiv_right ?_ (update_big_alloc (F:= F) (K := K) (V := (Agree (LeibnizO V)))
-      (Std.PartialMap.map (fun x => toAgree { car := x }) ∅)
-      (Std.PartialMap.map (fun x ↦ toAgree ⟨x⟩) m) (DFrac.own 1) ?_ ?_ ?_)
-    · refine CMRA.op_eqv ?_ (BigOpM.bigOpM_map_equiv _ _ _)
-      refine OFE.NonExpansive.eqv <| eqv_of_Equiv ?_
-      refine .trans ?_ LawfulPartialMap.union_empty_right
-      refine LawfulPartialMap.union_equiv PartialMap.equiv.refl LawfulPartialMap.map_empty
-    · simp only [EmptyCollection.emptyCollection, disjoint_iff, LawfulPartialMap.get?_map,
-      Option.map_eq_none_iff, get?_empty, Option.map_none, _root_.or_true, implies_true]
-    · exact DFrac.valid_own_one
-    · exact LawfulPartialMap.all_map fun _ _ => Agree.toAgree_valid
+    refine Update.equiv_right ?_
+      (update_big_alloc _ (Std.PartialMap.map (fun x ↦ toAgree ⟨x⟩) m) _
+        (disjoint_empty_right _) DFrac.valid_own_one
+        (all_map fun _ _ => Agree.toAgree_valid))
+    refine CMRA.op_eqv ?_ (BigOpM.bigOpM_map_equiv _ _ _)
+    exact OFE.NonExpansive.eqv (PartialMap.eqv_of_Equiv union_empty_right)
 
 @[rocq_alias ghost_map_alloc_strong_empty]
-theorem ghost_map_alloc_strong_empty [DecidableEq K] (P : GName → Prop) :
-  (∀ N, ∃ k, N ≤ k ∧ P k) →
-  ⊢@{IProp GF} |==> ∃ γ, ⌜P γ⌝ ∗ (γ ↪●MAP (∅ : H V)) := by
-  iintro %Hinf
+theorem ghost_map_alloc_strong_empty [DecidableEq K] (P : GName → Prop)
+    (Hinf : ∀ N, ∃ k, N ≤ k ∧ P k) :
+    ⊢@{IProp GF} |==> ∃ γ, ⌜P γ⌝ ∗ (γ ↪●MAP (∅ : H V)) := by
   imod ghost_map_alloc_strong P (∅ : H V) Hinf with ⟨%γ, H1, H2, -⟩
   iexists γ
   iframe
 
 @[rocq_alias ghost_map_alloc]
 theorem ghost_map_alloc [DecidableEq K] (m : H V) :
-  ⊢@{IProp GF} |==> ∃ γ, (γ ↪●MAP m) ∗
-    [∗map] k ↦ v ∈ m, γ ↪◯MAP[k] v := by
+    ⊢@{IProp GF} |==> ∃ γ, (γ ↪●MAP m) ∗ [∗map] k ↦ v ∈ m, γ ↪◯MAP[k] v := by
   imod (ghost_map_alloc_strong (fun _ => True) m) with ⟨%γ, -, H1, H2⟩
   · intro N; exists N; simp
   · iexists γ
     iframe H1 H2
 
 @[rocq_alias ghost_map_alloc_empty]
-theorem ghost_map_alloc_empty [DecidableEq K] :
-  ⊢@{IProp GF} |==> ∃ γ, (γ ↪●MAP (∅ : H V)) := by
+theorem ghost_map_alloc_empty [DecidableEq K] : ⊢@{IProp GF} |==> ∃ γ, (γ ↪●MAP (∅ : H V)) := by
   imod ghost_map_alloc (∅ : H V) with ⟨%γ, _, -⟩
   imodintro
   iexists γ
@@ -272,20 +261,19 @@ instance ghost_map_auth_fractional (m : H V) :
     rfl
 
 @[rocq_alias ghost_map_auth_as_fractional]
-instance (γ : GName) (m : H V) (q : F)
-    : AsFractional (PROP := IProp GF) (γ ↪●MAP{.own q} m)
-      (fun q => γ ↪●MAP{.own q} m) q where
+instance (γ : GName) (m : H V) (q : F) :
+    AsFractional (PROP := IProp GF) (γ ↪●MAP{.own q} m) (fun q => γ ↪●MAP{.own q} m) q where
   as_fractional := IProp.ext_iff.mp rfl
   as_fractional_fractional := ghost_map_auth_fractional m
 
 @[rocq_alias ghost_map_auth_valid]
 theorem ghost_map_auth_valid γ (dq : DFrac F) (m : H V) :
-  ⊢@{IProp GF} (γ ↪●MAP{dq} m) -∗ ⌜✓ dq⌝ := by
-    unfold ghost_map_auth
-    iintro _
-    refine iOwn_cmraValid.trans ?_
-    iintro %H; ipure_intro
-    apply auth_valid_iff.mp H
+    ⊢@{IProp GF} (γ ↪●MAP{dq} m) -∗ ⌜✓ dq⌝ := by
+  unfold ghost_map_auth
+  iintro _
+  refine iOwn_cmraValid.trans ?_
+  iintro %H; ipure_intro
+  apply auth_valid_iff.mp H
 
 @[rocq_alias ghost_map_auth_valid_2]
 theorem ghost_map_auth_valid_2 {γ} {dq1 dq2 : DFrac F} {m1 m2 : H V} :
@@ -297,9 +285,9 @@ theorem ghost_map_auth_valid_2 {γ} {dq1 dq2 : DFrac F} {m1 m2 : H V} :
   have ⟨h₁, h₂⟩ := auth_op_auth_valid_iff.mp G
   refine ⟨h₁, fun k => ?_⟩
   have h := h₂ k
-  simp only [LawfulPartialMap.get?_map, Option.map] at h
-  cases h₁ : get? m1 k <;> cases h₂ : get? m2 k
-    <;> grind [OFE.not_none_eqv_some, OFE.not_some_eqv_none,
+  simp only [get?_map, Option.map] at h
+  cases h₁ : get? m1 k <;> cases h₂ : get? m2 k <;>
+    grind [OFE.not_none_eqv_some, OFE.not_some_eqv_none,
       → Agree.toAgree_inj, LeibnizO.eqv_inj, OFE.some_eqv_some, Option.some.injEq]
 
 @[rocq_alias ghost_map_auth_agree]
@@ -310,13 +298,13 @@ theorem ghost_map_auth_agree γ (dq1 dq2 : DFrac F) (m1 m2 : H V) :
 
 @[rocq_alias ghost_map_auth_persist]
 theorem ghost_map_auth_persist γ dq (m : H V) :
-  ⊢@{IProp GF} (γ ↪●MAP{dq} m) ==∗ γ ↪●MAP{.discard} m := by
+    ⊢@{IProp GF} (γ ↪●MAP{dq} m) ==∗ γ ↪●MAP{.discard} m := by
   unfold ghost_map_auth
   iapply iOwn_update auth_dfrac_discard
 
 @[rocq_alias ghost_map_auth_unpersist]
 theorem ghost_map_auth_unpersist [IsHalfFraction F] γ (m : H V) :
-  ⊢@{IProp GF} (γ ↪●MAP{.discard} m) ==∗ ∃ q, γ ↪●MAP{.own q} m := by
+    ⊢@{IProp GF} (γ ↪●MAP{.discard} m) ==∗ ∃ q, γ ↪●MAP{.own q} m := by
   unfold ghost_map_auth
   iintro H
   imod iOwn_updateP auth_dfrac_acquire $$ H with ⟨%a, %Heq, G⟩
@@ -328,13 +316,13 @@ theorem ghost_map_auth_unpersist [IsHalfFraction F] γ (m : H V) :
 
 @[rocq_alias ghost_map_lookup]
 theorem ghost_map_lookup {γ dq} {m : H V} {k : K} {dq' v} :
-  ⊢@{IProp GF} (γ ↪●MAP{dq} m) -∗ (γ ↪◯MAP[k]{dq'} v) -∗ ⌜get? m k = some v⌝ := by
+    ⊢@{IProp GF} (γ ↪●MAP{dq} m) -∗ (γ ↪◯MAP[k]{dq'} v) -∗ ⌜get? m k = some v⌝ := by
   unfold ghost_map_auth ghost_map_elem
   iintro H1 H2
   icombine H1 H2 gives %G
   ipure_intro
   have ⟨av', _, _, h_av', _, h⟩ := auth_op_frag_valid_total_discrete_iff G
-  cases h₂ : get? m k <;> grind [Std.LawfulPartialMap.get?_map,Agree.toAgree_included, OFE.leibniz]
+  cases h₂ : get? m k <;> grind [get?_map,Agree.toAgree_included, OFE.leibniz]
 
 @[rocq_alias ghost_map_lookup_combine_gives_1]
 instance ghost_map_lookup_combine_gives_1 γ (m : H V) (k : K) (dq1 dq2 : DFrac F) (v : V) :
@@ -357,42 +345,39 @@ instance ghost_map_lookup_combine_gives_2 γ (m : H V) (k : K) (dq dq' : DFrac F
     ipure_intro; assumption
 
 @[rocq_alias ghost_map_insert]
-theorem ghost_map_insert {γ} {m : H V} (k : K) (v : V) :
-  get? m k = .none →
-  ⊢@{IProp GF} (γ ↪●MAP m) ==∗ (γ ↪●MAP insert m k v) ∗ γ ↪◯MAP[k] v := by
+theorem ghost_map_insert {γ} {m : H V} (k : K) (v : V) (Heq : get? m k = .none) :
+    ⊢@{IProp GF} (γ ↪●MAP m) ==∗ (γ ↪●MAP insert m k v) ∗ γ ↪◯MAP[k] v := by
   unfold ghost_map_auth ghost_map_elem
-  iintro %Heq H
-  imod iOwn_update (update_one_alloc (k := k) (v1 := toAgree (⟨v⟩ : LeibnizO V))
-    (by simp [LawfulPartialMap.get?_map, Heq])
+  iintro H
+  imod iOwn_update (update_one_alloc (k := k) (v1 := toAgree ⟨v⟩)
+    (by simp [get?_map, Heq])
     DFrac.valid_own_one
     (by simp [Agree.valid_def, Agree.valid, Agree.validN, toAgree])) $$ H with H
   icases H with ⟨H, $⟩
   imodintro
   iapply iOwn_mono $$ H
-  exact auth_inc_of_pmap_equiv _ LawfulPartialMap.map_insert
+  exact auth_inc_of_pmap_equiv _ map_insert
 
 @[rocq_alias ghost_map_insert_persist]
-theorem ghost_map_insert_persist {γ} {m : H V} (k : K) (v : V) :
-  get? m k = .none →
-  ⊢@{IProp GF} (γ ↪●MAP m) ==∗ (γ ↪●MAP insert m k v) ∗ (γ ↪◯MAP[k]{.discard} v) := by
-  iintro %Heq H
+theorem ghost_map_insert_persist {γ} {m : H V} (k : K) (v : V) (Heq : get? m k = .none) :
+    ⊢@{IProp GF} (γ ↪●MAP m) ==∗ (γ ↪●MAP insert m k v) ∗ (γ ↪◯MAP[k]{.discard} v) := by
+  iintro H
   imod ghost_map_insert k v Heq $$ H with ⟨$, G⟩
   iapply ghost_map_elem_persist $$ G
 
 @[rocq_alias ghost_map_delete]
 theorem ghost_map_delete {γ} {m : H V} (k : K) (v : V) :
-  ⊢@{IProp GF} (γ ↪●MAP m) -∗ (γ ↪◯MAP[k] v) ==∗ γ ↪●MAP delete m k := by
+    ⊢@{IProp GF} (γ ↪●MAP m) -∗ (γ ↪◯MAP[k] v) ==∗ γ ↪●MAP delete m k := by
   unfold ghost_map_auth ghost_map_elem
   iintro H1 H2
   icombine H1 H2 as G
-  imod iOwn_update (update_one_delete (k := k) (v1 := toAgree (⟨v⟩ : LeibnizO V)))
-    $$ G with G
+  imod iOwn_update (update_one_delete (k := k) (v1 := toAgree (⟨v⟩ : LeibnizO V))) $$ G with G
   iapply iOwn_mono $$ G
-  exact auth_inc_of_pmap_equiv _ LawfulPartialMap.map_delete
+  exact auth_inc_of_pmap_equiv _ map_delete
 
 @[rocq_alias ghost_map_update]
 theorem ghost_map_update {γ} {m : H V} (k : K) (v : V) (w : V) :
-  ⊢@{IProp GF} (γ ↪●MAP m) -∗ (γ ↪◯MAP[k] v) ==∗ (γ ↪●MAP insert m k w) ∗ γ ↪◯MAP[k] w := by
+    ⊢@{IProp GF} (γ ↪●MAP m) -∗ (γ ↪◯MAP[k] v) ==∗ (γ ↪●MAP insert m k w) ∗ γ ↪◯MAP[k] w := by
   iintro auth_m frag_kv
   ihave >aux := ghost_map_delete $$ auth_m frag_kv
   ihave >⟨aux, $⟩ := ghost_map_insert _ w (get?_delete_eq rfl) $$ aux
@@ -401,16 +386,13 @@ theorem ghost_map_update {γ} {m : H V} (k : K) (v : V) (w : V) :
   iapply iOwn_mono $$ aux
   refine auth_inc_of_pmap_equiv _ ?_
   intro i
-  rw [LawfulPartialMap.get?_map, LawfulPartialMap.get?_map,
-    LawfulPartialMap.insert_delete i]
+  rw [get?_map, get?_map, insert_delete i]
 
 /-! ### Big-op versions of the above lemmas -/
 
 @[rocq_alias ghost_map_lookup_big]
 theorem ghost_map_lookup_big {γ dq} {m : H V} {dq'} m0 :
-  ⊢@{IProp GF} (γ ↪●MAP{dq} m) -∗
-  ([∗map] k ↦ v ∈ m0, γ ↪◯MAP[k]{dq'} v) -∗
-  ⌜m0 ⊆ m⌝ := by
+    ⊢@{IProp GF} (γ ↪●MAP{dq} m) -∗ ([∗map] k ↦ v ∈ m0, γ ↪◯MAP[k]{dq'} v) -∗ ⌜m0 ⊆ m⌝ := by
   iintro H1 H2
   simp only [Subset, submap]
   iintro %k %v %Heq
@@ -418,48 +400,39 @@ theorem ghost_map_lookup_big {γ dq} {m : H V} {dq'} m0 :
   iapply BigSepM.bigSepM_lookup Heq $$ H2
 
 @[rocq_alias ghost_map_insert_big]
-theorem ghost_map_insert_big [DecidableEq K] {γ m} (m' : H V) :
-  (m' ##ₘ m) →
+theorem ghost_map_insert_big [DecidableEq K] {γ m} (m' : H V) (Hdisj : m' ##ₘ m) :
   ⊢@{IProp GF} (γ ↪●MAP m) ==∗
   (γ ↪●MAP (m' ∪ m)) ∗ [∗map] k ↦ v ∈ m', γ ↪◯MAP[k] v := by
   unfold ghost_map_auth ghost_map_elem
-  iintro %Hdisj H
+  iintro H
   by_cases h : m' ≡ₘ ∅
   · imodintro
     isplitl [H]
     · iapply iOwn_mono $$ H
-      refine auth_inc_of_pmap_equiv _ (fun i => ?_)
-      simp [LawfulPartialMap.get?_map, Union.union, get?_merge, h i,
-        EmptyCollection.emptyCollection, get?_empty]
+      exact auth_inc_of_pmap_equiv _ (map_equiv ((union_equiv h .refl).trans union_empty_left))
     · simp only [bigSepM]
       refine (BI.equiv_iff.mp ?_).mpr
       refine (BigOpM.bigOpM_equiv_of_perm _ h).trans ?_
       simp [BigOpM.bigOpM_empty]
-  rw [←IProp.ext (bigOpM_iOwn γ _ _ h), ←IProp.ext iOwn_op]
-  imod iOwn_update (E := GhostMapG.elem) (update_big_alloc _
-      (Std.PartialMap.map (fun x ↦ toAgree ⟨x⟩) m') (DFrac.own 1)
-      ?_ DFrac.valid_own_one ?_) $$ H with H
-  · intro i
-    specialize Hdisj i; simp only [not_and, Bool.not_eq_true, Option.isSome_eq_false_iff,
-      Option.isNone_iff_eq_none] at Hdisj
-    grind [LawfulPartialMap.get?_map]
-  · exact LawfulPartialMap.all_map fun _ _ => Agree.toAgree_valid
-  · icases H with ⟨H1, H2⟩
+  · rw [←IProp.ext (bigOpM_iOwn γ _ _ h), ←IProp.ext iOwn_op]
+    imod iOwn_update (E := GhostMapG.elem) (update_big_alloc _
+        (Std.PartialMap.map (fun x ↦ toAgree ⟨x⟩) m') (DFrac.own 1)
+        (disjoint_map Hdisj) DFrac.valid_own_one
+        (all_map fun _ _ => Agree.toAgree_valid)) $$ H with H
+    icases H with ⟨H1, H2⟩
     imodintro
     isplitl [H1]
     · iapply iOwn_mono $$ H1
-      exact auth_inc_of_pmap_equiv _ LawfulPartialMap.map_union
+      exact auth_inc_of_pmap_equiv _ map_union
     · iapply iOwn_mono $$ H2
       refine inc_of_inc_of_eqv .rfl ?_
       refine .trans ?_ (BigOpM.bigOpM_map_equiv _ _ _).symm
       exact .rfl
 
 @[rocq_alias ghost_map_insert_persist_big]
-theorem ghost_map_insert_persist_big [DecidableEq K] {γ m} (m' : H V) :
-  m' ##ₘ m →
-  ⊢@{IProp GF} (γ ↪●MAP m) ==∗
-  (γ ↪●MAP (m' ∪ m)) ∗ [∗map] k ↦ v ∈ m', γ ↪◯MAP[k]{.discard} v := by
-  iintro %Hdisj H
+theorem ghost_map_insert_persist_big [DecidableEq K] {γ m} (m' : H V) (Hdisj : m' ##ₘ m) :
+    ⊢@{IProp GF} (γ ↪●MAP m) ==∗ (γ ↪●MAP (m' ∪ m)) ∗ [∗map] k ↦ v ∈ m', γ ↪◯MAP[k]{.discard} v := by
+  iintro H
   imod ghost_map_insert_big m' Hdisj $$ H with ⟨$, H⟩
   iapply BigSepM.bigSepM_bupd
   iapply BigSepM.bigSepM_impl $$ H
@@ -468,62 +441,46 @@ theorem ghost_map_insert_persist_big [DecidableEq K] {γ m} (m' : H V) :
 
 @[rocq_alias ghost_map_delete_big]
 theorem ghost_map_delete_big [DecidableEq K] {γ m} (m0 : H V) :
-  ⊢@{IProp GF} (γ ↪●MAP m) -∗
-  ([∗map] k ↦v ∈ m0, γ ↪◯MAP[k] v) ==∗
-  (γ ↪●MAP (m \ m0)) := by
+    ⊢@{IProp GF} (γ ↪●MAP m) -∗ ([∗map] k ↦v ∈ m0, γ ↪◯MAP[k] v) ==∗ (γ ↪●MAP (m \ m0)) := by
   iintro H1 H2
   imod ghost_map_elems_unseal $$ H2 with H2
   unfold ghost_map_auth
   iapply iOwn_update_op $$ [$H1 $H2]
-  refine Update.equiv_left
-    (CMRA.op_right_eqv _
-      (BigOpM.bigOpM_map_equiv
-        (fun x : V => toAgree (LeibnizO.mk x))
-        (fun k v => Frag k (DFrac.own 1) v) m0))
-    ?_
+  refine Update.equiv_left (CMRA.op_right_eqv _ (BigOpM.bigOpM_map_equiv _ _ m0)) ?_
   refine (update_big_delete _ _).trans ?_
   refine Update.equiv_right ?_ .id
-  exact OFE.NonExpansive.eqv (PartialMap.eqv_of_Equiv LawfulPartialMap.map_difference_map)
+  exact OFE.NonExpansive.eqv (PartialMap.eqv_of_Equiv map_difference_map)
 
 @[rocq_alias ghost_map_update_big]
-theorem ghost_map_update_big [DecidableEq K] {γ m} (m0 m1 : H V) :
-  dom m0 = dom m1 →
-  ⊢@{IProp GF} (γ ↪●MAP m) -∗
-  ([∗map] k ↦v ∈ m0, γ ↪◯MAP[k] v) ==∗
-  (γ ↪●MAP (m1 ∪ m)) ∗ [∗map] k ↦ v ∈ m1, γ ↪◯MAP[k] v := by
-  iintro %Heq H1 H2
+theorem ghost_map_update_big [DecidableEq K] {γ m} (m0 m1 : H V) (Heq : dom m0 = dom m1) :
+    ⊢@{IProp GF} (γ ↪●MAP m) -∗ ([∗map] k ↦v ∈ m0, γ ↪◯MAP[k] v) ==∗
+    (γ ↪●MAP (m1 ∪ m)) ∗ [∗map] k ↦ v ∈ m1, γ ↪◯MAP[k] v := by
+  iintro H1 H2
   imod ghost_map_elems_unseal $$ H2 with H2
   by_cases h : m1 ≡ₘ ∅
   · imodintro
     isplitl [H1]
     · unfold ghost_map_auth
       iapply iOwn_mono $$ H1
-      refine auth_inc_of_pmap_equiv _ (fun i => ?_)
-      simp [LawfulPartialMap.get?_map, Union.union, get?_merge, h i,
-        EmptyCollection.emptyCollection, get?_empty]
+      exact auth_inc_of_pmap_equiv _ (map_equiv ((union_equiv h .refl).trans union_empty_left))
     · simp only [bigSepM]
       iclear H2
       refine (BI.equiv_iff.mp ?_).mpr
       refine (BigOpM.bigOpM_equiv_of_perm _ h).trans ?_
       simp [BigOpM.bigOpM_empty]
-  unfold ghost_map_elem ghost_map_auth
-  icombine H1 H2 as H
-  rw [←IProp.ext (bigOpM_iOwn γ _ _ h), ←IProp.ext iOwn_op]
-  iapply iOwn_update $$ H
-  refine Update.equiv_left
-    (CMRA.op_right_eqv _
-      (BigOpM.bigOpM_map_equiv
-        (fun x : V => toAgree (LeibnizO.mk x))
-        (fun k v => Frag k (DFrac.own 1) v) m0))
-    ?_
-  have Heq' : dom (Std.PartialMap.map (fun x : V => toAgree (LeibnizO.mk x)) m0)
-    = dom (Std.PartialMap.map (fun x : V => toAgree (LeibnizO.mk x)) m1) := by
-    rw [LawfulPartialMap.dom_map, LawfulPartialMap.dom_map, Heq]
-  refine (update_big_replace _ _ _ Heq'
-    (LawfulPartialMap.all_map fun _ _ => Agree.toAgree_valid)).trans ?_
-  refine Update.equiv_right ?_ .id
-  refine CMRA.op_eqv ?_ (BigOpM.bigOpM_map_equiv _ _ _)
-  exact OFE.NonExpansive.eqv (PartialMap.eqv_of_Equiv LawfulPartialMap.map_union.symm)
+  · unfold ghost_map_elem ghost_map_auth
+    icombine H1 H2 as H
+    rw [←IProp.ext (bigOpM_iOwn γ _ _ h), ←IProp.ext iOwn_op]
+    iapply iOwn_update $$ H
+    refine Update.equiv_left (CMRA.op_right_eqv _ (BigOpM.bigOpM_map_equiv _ _ m0)) ?_
+    have Heq' : dom (Std.PartialMap.map (fun x : V => toAgree (LeibnizO.mk x)) m0)
+      = dom (Std.PartialMap.map (fun x : V => toAgree (LeibnizO.mk x)) m1) := by
+      rw [dom_map, dom_map, Heq]
+    refine (update_big_replace _ _ _ Heq'
+      (all_map fun _ _ => Agree.toAgree_valid)).trans ?_
+    refine Update.equiv_right ?_ .id
+    refine CMRA.op_eqv ?_ (BigOpM.bigOpM_map_equiv _ _ _)
+    exact OFE.NonExpansive.eqv (PartialMap.eqv_of_Equiv map_union.symm)
 
 end lemmas
 
